$Tasks/Task3/removeNegatives.dfy
@@ -1,0 +1,30 @@
+datatype IntList =
+Nil
+| Cons(head: int, tail: IntList)
+
+function Length(l: IntList): nat
+{
+  match l
+  case Nil => 0
+  case Cons(_, t) => 1 + Length(t)
+}
+
+function Contains(l: IntList, x: int): bool
+{
+  match l
+  case Nil => false
+  case Cons(h, t) => h == x || Contains(t, x)
+}
+
+function RemoveNegatives(l: IntList): IntList
+  ensures forall x :: Contains(RemoveNegatives(l), x) ==> x >= 0
+  ensures Length(RemoveNegatives(l)) <= Length(l)
+{
+  match l
+  case Nil => Nil
+  case Cons(h, t) =>
+    if h < 0 then
+      RemoveNegatives(t)
+    else
+      Cons(h, RemoveNegatives(t))
+}
